update parser logic
add details to pre/postconditions for parsing methods. add helper functions for verifying input. update parsing functions expr, op, unaryOp, binaryOp, variableOp to use next_idx instead of shadowing current_idx

parser.dfy
@@ -1,4 +1,4 @@
-include "test.dfy" 
+//include "test.dfy" 
 //include "lexer.dfy" //TODO will uncomment these later once the files are unified
 
 /* more or less the grammar we're parsing
@@ -6,8 +6,8 @@ include "test.dfy"
 <expr>          ::= <unary-op> | <binary-op> | <variable-op> | <digits>
 <unary-op>      ::= (<unary> <expr>)
 <binary-op>     ::= (<binary> <expr> <expr>)
-<variable-op>   ::= (<variable> <expr> <expr-list>)
-<expr-list>     ::= <expr> <expr-list> | ε
+<variable-op>   ::= (<variable> <expr-list>)
+<expr-list>     ::= <expr> | <expr> <expr-list>
 <unary>         ::= abs | sqrt | ceil
 <binary>        ::= modulo | expt
 <variable>      ::= min | max | + | * | - | /
@@ -31,24 +31,24 @@ datatype Expr = Number(value: string)
               | BinaryOp(op:string, arg1: Expr, arg2: Expr)
               | VariableOp(op: string, arg1: Expr, argList: seq<Expr>)
 
-//result datatype will either allow us to store a value
-//or it will produce an error/failure
+//result datatype will either allow us to store a value or it will report an error/failure
 //has to be generic so we can store Expr or Token
 datatype Result<T> = Ok(data: T) | Err(error: string)
 
-
-//Helper functions
+//helper functions
+//true if the token provided represents a valid unary operation
 function isUnaryOp(operationType: TokenType, operationValue: string) : bool
 {
     operationType == TokenType.UNARY_OP &&
     (operationValue == "abs" || operationValue == "sqrt" || operationValue == "ceil")
 }
+//true if the token provided represents a valid binary operation
 function isBinaryOp(operationType: TokenType, operationValue: string) : bool
 {
     operationType == TokenType.BINARY_OP &&
     (operationValue == "modulo" || operationValue == "expt")
 }
-
+//true if the token provided represents a valid variable-argument operation
 function isVariableOp(operationType: TokenType) : bool
 {
     operationType == TokenType.VARIABLE_OP ||
@@ -57,93 +57,95 @@ function isVariableOp(operationType: TokenType) : bool
     operationType == TokenType.SLASH ||
     operationType == TokenType.MINUS
 }
+//true if the string provided is a valid operation in the language
+function isValidOp(operationValue: string): bool{
+    operationValue == "+" || operationValue == "-" ||
+    operationValue == "*" || operationValue == "/" ||
+    operationValue == "abs" || operationValue == "ceil" ||
+    operationValue == "modulo" || operationValue == "expt" ||
+    operationValue == "min" || operationValue == "max"
+}
 
+//helper predicates
+//TODO
+predicate ValidSubexpression(expr: Expr){
+    true
+}
+predicate ValidSubexpressions(exprs: seq<Expr>)
+{
+    forall i :: 0 <= i < |exprs| ==> ValidSubexpression(exprs[i])
+}
 
+//helper methods
+//peek ahead by a single token, but do not consume it
+//if there are no more tokens, return EOF
+method peekToken(tokens: seq<Token>, current_idx: int) returns (result: Token)
+requires 0 <= current_idx <= |tokens|
+ensures current_idx < |tokens| ==> result == tokens[current_idx]
+//if idx is out of bounds, just return EOF
+ensures current_idx == |tokens| ==> result.token_type == TokenType.EOF {
+    if current_idx == |tokens|{
+        var res := Pair(TokenType.EOF, "EOF");
+        return res;
+    }
+    result := tokens[current_idx];
+}
 
 //-------------------------------PARSING--------------------------------
 //transform a set of tokens into an AST
-//returns Err if expression is invalid 
-//otherwise returns Ok containing the AST root
+//returns Err if expression is invalid, otherwise returns Ok containing the AST root
 method parse(tokens: seq<Token>) returns (result: Result<Expr>)
 //preconditions
 //list of tokens should be nonempty
+//the lexer should add at least the EOF token at the end
 requires |tokens| > 0
-//postconditions
-//TODO add ensures...
-//TODO the index for the list should be at the end of the list, indicating all tokens were parsed
-//TODO should guarantee that the last token is EOF and was parsed
-//TODO should guarantee that all of the tokens were consumed into the tree
+//it must either parse the expression, or return an error
+ensures result.Ok? || result.Err?
+//this is kind of like return True? what to verify here?
 {
-    
     //parse starting at first token
-    var ast: Result<Expr>, current_idx: int := expr(tokens, 0);
+    var start_idx := 0;
+    var ast: Result<Expr>, end_idx: int := expr(tokens, start_idx);
+
+    //could not parse invalid expression
+    if ast.Err?{
+        assert end_idx <= |tokens|;
+        return ast;
+    }
+
+    //otherwise the expression was successfully parsed
+    assert ast.Ok?;
+    assert end_idx <= |tokens|;
 
     //last token should be the EOF token
-    //TODO prove these lines once parsing is done
-    //assert 0 <= current_idx < |tokens|;
-    //assert current_idx == |tokens| - 1;
-    assume{:axiom} 0 <= current_idx < |tokens|;
-    assume{:axiom} current_idx == |tokens| - 1;
+    assume{:axiom} end_idx == |tokens| - 1;
 
+    //TODO prove these lines once parsing is done
+    //assert 0 <= end_idx < |tokens|;
     //make sure that after parsing ends, the last token is EOF
+    //if it isn't we didn't parse it all the way
     //TODO not sure if we need to even do this
-    if tokens[current_idx].token_type != TokenType.EOF{
+    if tokens[end_idx].token_type != TokenType.EOF{
         return Err("unexpected end of file");
     }
 
-    current_idx := current_idx + 1;
-    assert current_idx == |tokens|;
+    //consume EOF
+    end_idx := end_idx + 1;
+    assert end_idx == |tokens|;
     return ast;
 }
 
-//parse an expression
-method expr(tokens: seq<Token>, current_idx: int) returns (result: Result<Expr>, end_idx: int)
-requires |tokens| > 0
-requires 0 <= current_idx < |tokens|
-ensures current_idx < end_idx //<= |tokens| //<-- TODO do we want this to hold
-decreases |tokens| - current_idx //think this fixes the termination issue
-//TODO add ensures
-{
-    //shadow current_idx
-    var current_idx := current_idx;
-
-    //get start at the next token
-    var next_token: Token := tokens[0];
-    var token_type := next_token.token_type;
-    var token_val := next_token.token_value;
-
-    //expression can be just a number
-    if token_type == TokenType.NUMBER{
-        result, end_idx := number(tokens, current_idx);
-    }
-    //parse some operation
-    else if token_type == TokenType.LEFT_PAREN{
-        //consume left parenthesis to get to operation
-        current_idx := current_idx + 1;
-
-        //will need this to pass
-        //TODO need to prove that current_idx + 1 <= |tokens|
-        //maybe use the advance_idx function somehow?
-        assume{:axiom} current_idx < |tokens|;
-        result, end_idx := op(tokens, current_idx);
-    }
-    //unrecognized token
-    else{
-        return Err("unrecognized expression"), current_idx + 1;
-    }
-}
-
-//consume the token at the current_idx
-//this token represents a number
+//return an expression representing a number
 method number(tokens: seq<Token>, current_idx: int) returns (result: Result<Expr>, end_idx: int)
-//should have at least one token to consume
 requires |tokens| > 0
 //our current idx should not be at the end of the list of tokens
 requires 0 <= current_idx < |tokens|
-//ensure that we consumed just one single token since it is a number
+//current token should be a number
+requires tokens[current_idx].token_type == TokenType.NUMBER
+//ensure that we consumed just the number token 
 ensures end_idx == current_idx + 1
-//ensure that we
-ensures end_idx <= |tokens| + 1
+//end index should still be in bounds
+ensures 0 <= end_idx <= |tokens|
 decreases |tokens| - current_idx 
 {
     //no other parsing needed than this
@@ -151,37 +153,87 @@ decreases |tokens| - current_idx
     return Ok(parsed_num), current_idx + 1;
 }
 
+//parse an expression
+method expr(tokens: seq<Token>, current_idx: int) returns (result: Result<Expr>, end_idx: int)
+//should be at least one token to parse
+requires |tokens| > 0
+//current_idx must be in bounds
+requires 0 <= current_idx < |tokens|
+//after parsing, end_idx should be within [0, len(tokens)]
+ensures 0 <= end_idx <= |tokens|
+//if we can parse the expression, the current_idx pointer must increase
+ensures result.Ok? ==> end_idx > current_idx
+decreases |tokens| - current_idx
+{
+    //get next token in list
+    var next_token: Token := tokens[current_idx];
+    var token_type := next_token.token_type;
+
+    //if the expression is a number, parse it
+    if token_type == TokenType.NUMBER{
+        var parsed_num, end_idx:= number(tokens, current_idx);
+        return parsed_num, end_idx;
+    }
+
+    //otherwise token is an expression
+    //subexpression should always start with '(', otherwise it's not a valid subexpression, e.g. "(+ 1 + 2 3)"
+    if next_token.token_type != TokenType.LEFT_PAREN{
+        //consume the invalid token, then return an error
+        var next_idx := current_idx + 1;
+        return Err("invalid expression"), next_idx;
+    }
+
+    //consume left parenthesis
+    var next_idx := current_idx + 1;
+
+    //check if the subexpression ends after the left parenthesis, e.g. "(+ 1 2 ("
+    if next_idx >= |tokens|{
+        return Err("unexpected end of file"), next_idx;
+    }
+
+    //parse the operation for expression
+    result, end_idx := op(tokens, next_idx);
+}
+
+
 
 //TODO dispatch to one of the operation-parsing functions based on token type
 method op(tokens: seq<Token>, current_idx: int) returns (result: Result<Expr>, end_idx: int)
+//should be at least one token
 requires |tokens| > 0
+//current_idx should be in bounds before parsing
 requires 0 <= current_idx < |tokens|
-//TODO might have to require this
-//requires current_idx < |tokens|-2
-//ensure that we consumed at least one token
-ensures end_idx > current_idx
-ensures end_idx <= |tokens| + 1
+//parser consumed at least one token
+ensures current_idx < end_idx <= |tokens|
+//if we can parse the operation, current_idx must increase
+ensures result.Ok? ==> end_idx > current_idx
 decreases |tokens| - current_idx
 {
-    var tokens := tokens;
-    var current_idx := current_idx;
-   
-    //verify that the next token is a valid operation token
-    //TODO
-
+    //starting token should be an operation 
     //extract the operation type from the current token
     var operation_type: TokenType := tokens[current_idx].token_type;
     var operation_value: string := tokens[current_idx].token_value;
-    
-    //TODO need to fix decreases clause because the program doesn't think our program terminate
+
+    //consume the operator
+    var next_idx := current_idx + 1;
+
+    //verify that the next token is a valid operation token
+    if !isValidOp(operation_value){
+        return Err("unknown operation"), next_idx;
+    }
+    //if there are no tokens after operator, invalid expression, e.g. "(+ 1 2 (+"
+    if next_idx >= |tokens|{
+        return Err("unexpected EOF"), next_idx;
+    }
+
     if operation_type == TokenType.UNARY_OP{
-        result, end_idx := unaryOp(tokens, current_idx, operation_value);
+        result, end_idx := unaryOp(tokens, next_idx, operation_value);
     }
     else if operation_type == TokenType.BINARY_OP{
-        result, end_idx := binaryOp(tokens, current_idx, operation_value);
+        result, end_idx := binaryOp(tokens, next_idx, operation_value);
     }
     else if isVariableOp(operation_type) {
-        result, end_idx := variableOp(tokens, current_idx, operation_value);
+        result, end_idx := variableOp(tokens, next_idx, operation_value);
     }
     else{
         result, end_idx := Err("invalid operation"), current_idx + 1;
@@ -189,106 +241,166 @@ decreases |tokens| - current_idx
 
 }
 
-//TODO parse a single unary operation starting at token with index current_idx
+//TODO parse a single unary operation
 method unaryOp(tokens: seq<Token>, current_idx: int, operation: string) returns (result: Result<Expr>, end_idx: int)
+//at least one token to parse
 requires |tokens| > 0
-requires 0 <= current_idx < |tokens|
-ensures current_idx < end_idx <= |tokens| + 1
-decreases |tokens| - current_idx //i think this fixes the termination issue?
+//current_idx is in bounds
+requires 0 < current_idx < |tokens|
+//after parsing, end_idx is still in bounds
+ensures current_idx < end_idx <= |tokens|
+//if we can parse the unary operation, current_idx must increase
+ensures result.Ok? ==> end_idx > current_idx
+decreases |tokens| - current_idx
 {
     //parse the expression after the operator
-    var parsed_subexpr, current_idx := expr(tokens, current_idx);
+    var parsed_subexpr, next_idx := expr(tokens, current_idx);
 
     //check if parsing the subexpression fails
     if parsed_subexpr.Err?{
-        return parsed_subexpr, current_idx;
+        return parsed_subexpr, next_idx;
+    }
+    //check if the expression ends without a right_paren, e.g. (+ 1 2 (* 3 4)
+    if next_idx >= |tokens|{
+        return Err("unexpected EOF"), next_idx;
+    }
+    //last token in expression should be a right paren
+    if tokens[next_idx].token_type != TokenType.RIGHT_PAREN{
+        return Err("missing RIGHT_PAREN"), next_idx;
     }
 
-    //else successfully parsed
+    //otherwise the operation can be parsed
     var parsed_unary_op := Ok(UnaryOp(operation, parsed_subexpr.data));
 
     //consume right parenthesis
-    current_idx := current_idx + 1;
-
     //return parsed unary op
-    result, end_idx := parsed_unary_op, current_idx;
+    result, end_idx := parsed_unary_op, next_idx + 1;
 }
 
 //TODO parse a single binary operation starting at token with index current_idx
 method binaryOp(tokens: seq<Token>, current_idx: int, operation: string) returns (result: Result<Expr>, end_idx: int)
+//should be at least one token to parse
 requires |tokens| > 0
+//current_idx should be in bounds
 requires 0 <= current_idx < |tokens|
-ensures current_idx < end_idx <= |tokens|+1
+//after parsing, end_idx should be in bounds
+ensures current_idx < end_idx <= |tokens|
+//if we can parse the binary operation, the index pointer must increase
+ensures result.Ok? ==> end_idx > current_idx
 decreases |tokens| - current_idx
 {
-    var current_idx := current_idx;
-    var parsed_subexpr_1: Result<Expr>, parsed_subexpr_2: Result<Expr>;
+    //parse the first subexpressions after the operator
+    var parsed_subexpr_1: Result<Expr>, next_idx: int;
+    parsed_subexpr_1, next_idx := expr(tokens, current_idx);
 
-    //parse the first expression after the operator
-    parsed_subexpr_1, current_idx := expr(tokens, current_idx);
-    //return error immediately if the subexpresion cannot be parsed
+    //check if parsing the subexpression fails
     if parsed_subexpr_1.Err?{
-        return parsed_subexpr_1, current_idx;
+        return parsed_subexpr_1, next_idx;
+    }
+    //check if the first subexpression ends without a right_paren, e.g. "(+ 1 (ceil 4.5" 
+    if next_idx >= |tokens|{
+        return Err("unexpected EOF"), next_idx;
     }
 
-    //parse the second expression after the operator
-    parsed_subexpr_2, current_idx := expr(tokens, current_idx);
-    //return error immediately if second subexpression cannot be parsed
+    assert next_idx < |tokens|;
+
+    //parse the second subexpressions after the operator
+    var parsed_subexpr_2: Result<Expr>;
+    parsed_subexpr_2, next_idx := expr(tokens, next_idx);
+
+    //check if parsing the second subexpression fails
     if parsed_subexpr_2.Err?{
-        return parsed_subexpr_2, current_idx;
+        return parsed_subexpr_2, next_idx;
+    }
+    //check if the second subexpression ends without a right_paren, e.g. "(+ 1 2 (* 3 4"
+    if next_idx >= |tokens|{
+        return Err("unexpected EOF"), next_idx;
     }
 
-    //make a binary operation using the current operation
-    var parsed_binary_op := BinaryOp(operation, parsed_subexpr_1.data, parsed_subexpr_2.data);
+    //after parsing both arguments, last token in expression should be a right paren
+    if tokens[next_idx].token_type != TokenType.RIGHT_PAREN{
+        return Err("missing RIGHT_PAREN"), next_idx;
+    }
 
     //consume right parenthesis
-    current_idx := current_idx + 1;
+    next_idx := next_idx + 1;
+
+    //make a binary operation using the current operation and two parsed subexpressions
+    var parsed_binary_op := BinaryOp(operation, parsed_subexpr_1.data, parsed_subexpr_2.data);
 
     //return parsed binary operation
-    result, end_idx := Ok(parsed_binary_op), current_idx;
+    result, end_idx := Ok(parsed_binary_op), next_idx;
 }
 
 //TODO parse a single variable-param operation starting at token with index current_idx
 method variableOp(tokens: seq<Token>, current_idx: int, operation: string) returns (result: Result<Expr>, end_idx: int)
+//should be at least one token to parse
 requires |tokens| > 0
+//current_idx should be valid
 requires 0 <= current_idx < |tokens|
-ensures current_idx < end_idx <= |tokens| + 1 
+//after parsing, should be at the end of the expression or in bounds 
+ensures current_idx < end_idx <= |tokens|
+//if the operation can be parsed, current_idx must increase
+ensures result.Ok? ==> end_idx > current_idx 
 decreases |tokens| - current_idx
 {
-    //shadow current_idx
-    var current_idx := current_idx;
-    var parsed_subexpr_1: Result<Expr>;
+    //required to have at least one subexpression after operator
+    var parsed_required_subexpression: Result<Expr>, next_idx: int;
 
     //parse required expressions after operator
-    parsed_subexpr_1, current_idx := expr(tokens, current_idx);
-    if parsed_subexpr_1.Err?{
-        return parsed_subexpr_1, current_idx;
+    parsed_required_subexpression, next_idx:= expr(tokens, current_idx);
+    if parsed_required_subexpression.Err?{
+        return parsed_required_subexpression, current_idx;
+    }
+    //check if the required subexpression ends without a right_paren, e.g. "(+ 1 2 (* 3 4"
+    if next_idx >= |tokens|{
+        return Err("unexpected EOF"), next_idx;
     }
 
-    //populate list of any remaining arguments
+    //populate argument list with any remaining arguments
     var subexprList: seq<Expr> := [];
-    //TODO figure out this loop
-    // while false
-    // invariant false
-    // {
-    //     //parse remaining args
-    //     //look ahead to next token
-    //     //if it is a RIGHT_PARENT, end of expression. loop terminates
-    //     //otherwise, keep parsing subexpressions and adding to list
-    // }
 
-    var parsed_variable_op := VariableOp(operation, parsed_subexpr_1.data, subexprList);
+    //look ahead to next token
+    //if it is a RIGHT_PARENT, end of expression. loop terminates
+    //otherwise, keep parsing subexpressions and adding to list
+    var nextToken: Token := peekToken(tokens, next_idx);
+    while nextToken.token_type != TokenType.RIGHT_PAREN
+    //current_idx is always in bounds
+    invariant 0 <= current_idx < |tokens|
+    //current_idx pointer always gets closer to the end of the token sequence
+    decreases |tokens| - current_idx
+    {
+        //parse next subexpr
+        var next_parsed_subexpr: Result<Expr>;
+        next_parsed_subexpr, next_idx:= expr(tokens, next_idx);
+        //check if subexpression can't be parsed
+        if next_parsed_subexpr.Err?{
+            return next_parsed_subexpr, current_idx;
+        }
+        //ensure that we are not at the end of the expression prematurely
+        if next_idx >= |tokens|{
+            return Err("unexpected EOF"), next_idx;
+        }
+
+        //add to list of arguments
+        subexprList := subexprList + [next_parsed_subexpr.data];
+
+        //move to next token in expression
+        nextToken := peekToken(tokens, current_idx);
+    }
+
+    var parsed_variable_op := VariableOp(operation, parsed_required_subexpression.data, subexprList);
 
     //consume right parenthesis
-    current_idx := current_idx + 1;
+    next_idx := next_idx + 1;
 
     //return parsed variable-argument operation
-    result, end_idx := Ok(parsed_variable_op), current_idx;
+    result, end_idx := Ok(parsed_variable_op), next_idx;
 }
 
 method main()
 requires true
 ensures true
 {
-    //TODO add something here maybe?
+    //TODO add something here
 }
